\documentclass[10pt]{extarticle}
\input{../../hw_preamble.tex}
\title{DEPT 10100: Homework 1}
\author{First Last}
\date{\today}
\email{first.last@university.edu}
\idnum{School ID \#: 000001}


\begin{document}


% Question environment example
\begin{question}[10pts]
    Let $X_1 \sim \text{Gamma}(r_1, \lambda)$ and $X_2 \sim \text{Gamma}(r_2, \lambda)$ be independent random variables, and let $Y = X_1 + X_2$ and let $Z = X_1 / (X_1 + X_2)$.
    Find the joint density of $Y$ and $Z$, and find the marginal densities of $Y$ and $Z$. Identify the distributions of $Y$ and $Z$. Note that $\text{Gamma}(r, \lambda)$ distribution has density function
        \begin{equation*}
            f(x)=\frac{\lambda^{r}}{\Gamma(r)} e^{-\lambda x} x^{r-1}, \quad x>0
        \end{equation*}
\end{question}
% Answer environment example
\begin{ans}
    Since $X_1 \indep X_2$, their joint density is the product of their marginal densities.
    \begin{equation}
        f_{X_1, X_2}(x_1, x_2) = \frac{\lambda^{r_1 + r_2}}{\Gamma(r_1) \cdot \Gamma(r_2)}\cdot  e^{-\lambda(x_1 + x_2)} \cdot x_1^{r_1 - 1} \cdot x_2^{r_2 - 1}
    \end{equation}
    Let $X = [X_1, X_2]^\intercal$. Define
    \begin{equation}
        \begin{bmatrix}
            Y \\
            Z \\
        \end{bmatrix} = H(X) = \begin{bmatrix}
            X_1 + X_2 \\
            \frac{X_1}{X_1 + X_2}
        \end{bmatrix}
    \end{equation}
    The transformation $H(X)$ has Jacobian matrix
    \begin{equation}
        J(H) = \begin{bmatrix}
            1 & 1 \\
            \frac{X_2}{(X_1 + X_2)^2} & \frac{-X_1}{(X_1 + X_2)^2}
        \end{bmatrix}
    \end{equation}
    the determinant of which is $-1 / (X_1 + X_2)$. So
    \begin{align}
        F_{Y, Z}(y, z) &= \sum_{X : H(X) = [y, z]} \frac{\lambda^{r_1 + r_2}}{\Gamma(r_1) \cdot \Gamma(r_2)}\cdot  e^{-\lambda(x_1 + x_2)} \cdot x_1^{r_1 - 1} \cdot x_2^{r_2 - 1} \cdot \underbrace{(x_1 + x_2)}_{=1 / \abs{\det(J(H))}} \\
                       &= \frac{\lambda^{r_1 + r_2}}{\Gamma(r_1) \cdot \Gamma(r_2)} \cdot e^{-\lambda(x_1 + x_2)} \cdot x_1^{r_1} \cdot x_2^{r_2} \cdot \frac{x_1 + x_2}{x_1 x_2} \\
                       &= \frac{\lambda^{r_1 + r_2}}{\Gamma(r_1) \cdot \Gamma(r_2)} \cdot e^{-\lambda y} \cdot (yz)^{r_1} \cdot (y(1 -z))^{r_2} \cdot \frac{1}{yz(1-z)} \\
                       &= \underbrace{\frac{\lambda^{r_1 + r_2}}{\Gamma(r_1 + r_2)} \cdot e^{-\lambda y} \cdot y^{r_1 + r_2 - 1}}_{\text{Gamma}(r_1 + r_2, \lambda)} \cdot \underbrace{\frac{\Gamma(r_1 + r_2)}{\Gamma(r_1) \cdot \Gamma(r_2)} \cdot z^{r_1 - 1} (1 - z)^{r_2 - 1}}_{\text{Beta}(r_1, r_2)} \label{eqn:1a1}
    \end{align}
    So~\ref{eqn:1a1} is the joint probability density of $Y$ and $Z$. Then, we integrate out $y$ and $z$ to obtain their marginal densities. First, note that $y$ has support in $[0, \infty)$, whereas $z$ has support in $(0, 1)$. Next, as the underbraced portions of~\ref{eqn:1a1} note, the joint probability density of $Y$ and $Z$ is the product of two expressions, one in $y$, the other in $z$, each of which is a known probability density. So
    \begin{align}
        f_Y(y) &= \frac{\lambda^{r_1 + r_2}}{\Gamma(r_1 + r_2)} \cdot e^{-\lambda y} \cdot y^{r_1 + r_2 - 1} \cdot \int_0^1 \frac{\Gamma(r_1 + r_2)}{\Gamma(r_1) \cdot \Gamma(r_2)} \cdot z^{r_1 - 1} (1 - z)^{r_2 - 1} dz \\
               &= \frac{\lambda^{r_1 + r_2}}{\Gamma(r_1 + r_2)} \cdot e^{-\lambda y} \cdot y^{r_1 + r_2 - 1}
    \end{align}
    and
    \begin{align}
        f_Z(z) &= \frac{\Gamma(r_1 + r_2)}{\Gamma(r_1) \cdot \Gamma(r_2)} \cdot z^{r_1 - 1} (1 - z)^{r_2 - 1} \cdot \int_0^\infty \frac{\lambda^{r_1 + r_2}}{\Gamma(r_1 + r_2)} \cdot e^{-\lambda y} \cdot y^{r_1 + r_2 - 1} dy \\
               &= \frac{\Gamma(r_1 + r_2)}{\Gamma(r_1) \cdot \Gamma(r_2)} \cdot z^{r_1 - 1} (1 - z)^{r_2 - 1}
    \end{align}
    So $Y \sim \text{Gamma}(r_1 + r_2, \lambda)$ and $Z \sim \text{Beta}(r_1, r_2)$. Furthermore, since $f_{Y, Z}(y, z) = f_{Y}(y) \cdot f_Z(z)$, $Y \indep Z$.
\end{ans}

% Code example
\begin{minted}[breaklines, linenos]{python}
def egyptian_multiplication(a, n):
    """
    Returns the product `a * n`.
    Assume n is a nonegative integer
    """

    def is_odd(n):
        """
        Returns True if n is odd.
        """
        return n & 0x1 == 1

    if n == 1:
        return a
    if n == 0:
        return 0

    if is_odd(n):
        return egyptian_multiplication(a + a, n // 2) + a
    else:
        return egyptian_multiplication(a + a, n // 2)
\end{minted}


% Todo box example
\todo

% Todo box example with optional argument
\todo[message]


\end{document}
